src/lib/kernel/gemm/Kuiper.Kernel.GEMM.Copy.Vec2.fsti
@@ -74,6 +74,7 @@ fn split_array2_into_strided_chunks
   (nthr : pos)
   requires
     m |-> em
+  ensures array_exists (core m)
   ensures
     pure (SZ.fits (l.ulen))
   ensures
@@ -88,6 +89,7 @@ fn join_array2_from_strided_chunks
   (m : array2 et l)
   (#em : chest2 et rows cols)
   (nthr : pos)
+  requires array_exists (core m)
   requires
     pure (SZ.fits (l.ulen))
   requires
@@ -103,6 +105,7 @@ fn join_array2_from_strided_chunks_underspec
   (#l : layout2 rows cols)
   (m : array2 et l)
   (nthr : pos)
+  requires array_exists (core m)
   requires
     pure (SZ.fits (l.ulen))
   requires
